## Sugar:

> \begin{aligned}
\because\quad
\mathcal{G}_g^{3D} 
&= \exp\!\left(-\frac{1}{2}(p-\mu_g)^T\Sigma^{-1}(p-\mu_g)\right) \\
&= \exp\!\left(-\frac{1}{2}\left(
\frac{1}{s_g^2}\langle p-\mu_g, u_g \rangle^2 +
\frac{1}{s_g^2}\langle p-\mu_g, v_g \rangle^2 +
\frac{1}{s_g^2}\langle p-\mu_g, n_g \rangle^2
\right)\right) \\
\mathcal{G}_g^{1D}
&\approx \exp\!\left(-\frac{1}{2s_g^2}\langle p-\mu_g, n_g \rangle^2
\right) \\
&= \exp\!\left(-\frac{1}{2s_g^2} f(p)^2\right) \\
\therefore\quad
f(p) &= \pm s_g\sqrt{-2\log\!\left(\mathcal{G}_g^{1D}\right)}
\to \text{Surface}
\end{aligned}







